# Expanding Algebraic Expressions

# Binomial Expansion

![image.png](Expanding%20Algebraic%20Expressions%20c71038bc5eec4535be64d706e08cf4b4/image.png)

- The diagram shows that $(a+b)(c+d) = ac+ad+bc+bd$
- Where
    - The expression in the brackets is the factorised.
    - The expression without the brackets is the expanded form.

![image.png](Expanding%20Algebraic%20Expressions%20c71038bc5eec4535be64d706e08cf4b4/image%201.png)

- The diagram shows that $(x+3)(x+2) = x^2+2x+3x+6  = x^2+5x+6$
- Where
    - The one is the brackets is the factorised form.
    - The one without the brackets is the expanded form.

# Example

Expand $(x-7)(6-x)$

$$
(x\times 6)+(x\times -x) +(-7\times 6) +(-7\times -x) \\  = 6x - x^2 - 42 +7x \\ = -x^2+13x - 42
$$

# Squaring Binomial Expressions

$$
(a+b)^2=a^2+2ab+b^2
$$

Similarly,

$$
(a-b)^2 = a^2-2ab+b^2
$$

- This expansion can be memorised by:
    - squaring the first term
    - multiply the two terms together and then double the product
    - square the last term

# Example

Expand and simplify $-2(2x+7)^2$

$$
= -3[(2x)^2+28x + 7^2] \\ = -3(4x^2+28x+7^2) \\ = - 12x^2 - 84x - 147
$$

# The difference of two Squares

- When $(a+b)$ is multiplied by $(a-b)$ (or vice-versa).

$$
(a+b)(a-b) = a^2-b^2
$$

# Example

Simplify $(3x+1)(3x-1)$\

$$
= (3x)^2-(1)^2 \\ = 9x^2-1
$$

Simplify $4(2x-7)(2x+7)$

$$
=4[(2x)^2-(7)^2] \\ = 4(4x^2-49) \\ = 16x^2 - 196
$$