# Factorising Expressions with two or four terms

- To factorise an expression with 2 terms use the following steps:
1. Look for the highest common factor (HCF) of the terms
2. Take out the HCF.
3. Check to see if the remaining expression is a DOTS.
- For example

$$
4x^2-36 = 4(x^2-9) \\ = 4(x-3)(+3)
$$

- Remember to use the formula for the difference of two squares:

$$
a^2-b^2 = (a-b)(a+b)
$$

# Example

Factorise $12k^2+18$

$$
= 6(2k^2+3)
$$

Factorise $16a^2 - 25b^4$

$$
= 4^2a^2 - 5^2(b^2)^2 \\ = (4a)^2 - (5b^2)^2 \\ = (4a+5b^2)(4a-5b^2)

$$

# Factorising with four terms

- To factorise an expression with four terms, follow the following steps:
1. look for a common factor
2. group in pairs that have a common factor
3. factorise each pair by taking out the common factor
4. factorise fully by taking out the common binomial factor

# Example

Factorise $10a-30b+15ac-45bc$

1. terms have a common factor of 5
2. grouping in pairs
3. factorising each pair
4. common binomial factor

$$
= 5(2a-6b+3ac-9bc) \\ =5(2(a-3b)+3c(a-3b)) \\ =5(a-3b)(2+3c)
$$

Factorise $x - 4y +mx-4my$

$$
=(x-4y)+(mx-4my) \\ = 1(x-4y)+m(x-4y) \\ = (x-4y)(1+m)
$$

Factorise $x^2+3x-y^2+3y$

Factorise by removing the common binomial factor in this case it is (x+y).

$$
= (x^2-y^2) + (3x+3y) \\ = (x+y)(x-y)+3(x+y) \\ =(x+y)(x-y+3)
$$