# Factorising Expressions with Three Terms

# Factorising monic quadratic trinomials

- A monic quadratic expression is an expression in the form $ax^2+bx+c$ where $a = 1$.
- To factorise a monic quadratic expression $x^2+bx+c$ we need to determine the numbers $f$ and $h$  such that $x^2 + bx+c = (x+f)(x+h)$

$$
(x+f)(x+h) = x^2+xh+xf+fh \\ = x^2+x(h+f)+fh
$$

- There fore when factorising a quadratic expression we must determine the factors of $c$ that add up to $b$.
- For example, to factrosie $x^2+7x+12$ we must determine the factors of 12 that add up to 7.

| Factors of 12 | Sum of Factors |
| --- | --- |
| 1 and 12 | 13 |
| 2 and 6 | 8 |
| 3 and 4 | 7 |
- The factors of 12 that add up to 7 are 3 and 4. Therefore, $x^2+7x+12 = (x+3)(x+4)$

## Factorising a monic quadratic

$$
x^2+bx+c = (x+f)(x+h)
$$

- Where $f$ and $h$ are factors of $c$ that sum up to $b$.

# Example

Factorise $x^2+10x+24$

To factorise this find the factors of 24 that add up to 10:

| Factors of 24 | Sum of Factors |
| --- | --- |
| 1 and 24 | 25 |
| 2 and 12 | 14 |
| 3 and 8 | 11 |
| 4 and 6 | 10 |

$$
=x^2+10x+24 \\= (x+4)(x+6)
$$

# Factorising Non-Monic Quadratic Trinomials

- Quadratic expressions of the form $ax^2+bx+c$ can be factorised by following the process shown below.
- For example: $2x^2+11x+12$
    1. Determine factors of $ac$ that add up to $b.$
    
    $$
    a = 2, \ b =11, \ c = 12, \ ac = 24
    $$
    
    The factors of 24 that add up to 11 are 8 and 3.
    
    1. Rewrite the quadratic expression as $ax^2+mx+nx+c$, where $m$ and $n$ are the factors of $ac$ that add up to $b$ (as found in step 1).
    
    $$
    2x^2 +11x+12 = 2x^2+8x+3x+12
    $$
    
    1. Order the terms in $ax^2+mx+nx+c$ so that the two terms on the left share a common factor and the two terms on the right also share a common factor.
    
    $$
    = (2x^2+8x)+(3x+12)
    $$
    
    1. Factorise the two left terms and the two right terms independently by taking out their common factor.
    
    $$
    = 2x(x+4)+3(x+4)
    $$
    
    1. Factorise the expression by taking out the binomial factor.
    
    $$
    = (2x+3)(x+4)
    $$
    

## Factorising a non-monic quadratic

- To factorise a general quadratic of the form $ax^2+mx+nx+c$, find factors of $ac$ that sum to $b$. Then rewrite the expression as four terms that can then be regrouped and factorised.

$$
ax^2+bx+c = ax^2+mx+nx+c
$$

Where $m$ and $n$ are factors of $ac$ that sum to $b$.

# Example

Factorise $6x^2 - 11x - 10$.

To factorise this find the factors of $ac$ that add up to $b$

$$
a = 6, \ c = -10 \\ \therefore ac =  -60
$$

| Factors of -60 | Sum of factors |
| --- | --- |
| -60 and 1 | -59 |
| -20 and 3 | -17 |
| -30 and 2 | -28 |
| 15 and -4 | 11 |
| -15 and 4 | -11 |

$$
= 6x^2-15x+4x+-10 \\ = (6x^2+4x)+(-15x+-10) \\ = 2x(3x+2)+-5(3x+2) \\ =(3x+2)(2x-5)
$$

Factorise $2x^2+x-6$

$$
2x^2+x-6 \\
$$

![image.png](c38608ff-9ad7-45d4-8edf-6f9e633cfe33.png)

$$
(
$$

Factorise $2x^2+7x+3$

Multiple $2 \times 3 = 6$ now find factors of 6 that add to 7

| Factors of 6 | sum |
| --- | --- |
| 6 and 1 | 7 |

$$
2x^2+6x+1x+3 \\ 2x(x+3)+1(x+3) \\ (x+3)(2x+1)
$$

Factorise $6x^2+5x-6$

Multiple $6 \times 6 = 36$ now find factors of 36 that add to or subtract to 5

| Factors of 36 | sum and difference |
| --- | --- |
| 6 and 6 | 12 and 0 |
| 12 and 3 | 15 and 9 |
| 9 and 4 | 13 and 5 |

$$
6x^2+9x-4x-6 \\ 3x(2x+3)-2(2x+3) \\ (3x-2)(2x+3)
$$