# Operations with Surds

## Multiplying and Simplifying Surds

## Multiplication of Surds

- In order to multiply two or more surds, use the following:

$$
\sqrt{a} \cdot \sqrt{b} = \sqrt{a\cdot b}
$$

$$
m\sqrt{a} \cdot n\sqrt{b} = mn\sqrt{a\cdot b}
$$

## Simplification of Surds

- To simplify a surd means to make the number under the radical sign as small as possible.
- Surds can only be simplified if the number under the radical sign has factor which is perfect square (4, 9, 16, 25, 36).
- The process to simplify a surd:
    - Split the number under the radical into the product of two factors, one of which is a perfect square.
    - Write the surd as the product of two surds multiplied together. The two surds must correspond to the factors identified in step 1.
    - Simplify the surd of the perfect square and write the surd in the form $a\sqrt{b}$.
- E.g.

$$
\sqrt{45} = \sqrt{9 \cdot5} \\ \hspace{10.8mm}= \sqrt{9} \cdot \sqrt{5} \\ \hspace{8mm} = 3 \cdot \sqrt{5} \\ \hspace{6mm} = 3\sqrt{5}
$$

## Example

Simplify $-\frac{1}{8}\sqrt{175}$

$$
=-\frac{1}{8} \sqrt{25\cdot7} \\ \hspace{5.5mm} = -\frac{1}{8} \cdot \sqrt{25} \cdot \sqrt{7} \\  = -\frac{1}{8} \cdot 5 \sqrt{7} \\ \therefore = -\frac{5}{8} \sqrt{7} 
$$

Simplify $5\sqrt{180x^{3}y^{5}}$

$$
\hspace{4mm}= 5\sqrt{36 \cdot 5 \cdot x^{2}\cdot x \cdot y^{4} \cdot y}
$$

$$
= 5\cdot \sqrt{36x^{2}y^{4}} \cdot \sqrt{5xy}
$$

$$
= 5 \cdot 6\cdot x \cdot y^{2} \cdot \sqrt{5xy}
$$

$$
= 30xy^{2}\sqrt{5xy}
$$

Solve $6\sqrt{12}\cdot2\sqrt{6}$

$$
=6\sqrt{4\cdot3}\cdot2\sqrt{6}
$$

$$
= 6\cdot2\sqrt{3}\cdot2\sqrt{6}
$$

$$
=12\sqrt{3}\cdot2\sqrt{6}
$$

$$
=24\sqrt{18}
$$

$$
=24\sqrt{9\cdot2}
$$

$$
=24\cdot3\sqrt{2}
$$

$$
=72\sqrt{2}
$$

## Squaring Surds

- When a surd is squared, the result is the expression under the radical sign:

$$
(\sqrt{a})^{2}=a
$$

## Example

Simplify $(3\sqrt{5})^{2}$

$$
=3^{2}\cdot(\sqrt{5})^{2}
$$

$$
=9\cdot5
$$

$$
=45
$$

## Addition and Subtraction of Surds

- Surds may be added or subtracted only if the surd are alike.
- It is best if you think of adding or subtracting surds as if you are combining like terms in algebra.
    
    $$
    2x \ + 12x = 14x 
    $$
    

$$
4\sqrt{3} \ + 4\sqrt{3} =8\sqrt{3}
$$

## Example

Simplify $5\sqrt{3} +2\sqrt{12}-5\sqrt{2}+3\sqrt{8}$

$$
= 5\sqrt{3} + 2\sqrt{4\times3} - 5\sqrt{2} + 3\sqrt{4\times2} \\ \hspace{0.3mm}= 5\sqrt{3} + 2 \times 2\sqrt{3} - 5\sqrt{2} + 3 \times 2\sqrt{2} \\ = 5\sqrt{3}+4\sqrt{3}-5\sqrt{2}+6\sqrt{2} \\ = 9\sqrt{3}+\sqrt{2}
$$

Simplify $\frac{1}{2}\sqrt{100a^{3}b^{2}}+ab\sqrt{36a}-5\sqrt{4a^{2}b}$

$$
= \frac{1}{2}\times10\sqrt{a^{2}\times a\times b^{2}}+ab\times6\sqrt{a}-5\times2\times a\sqrt{b} \\ = \frac{1}{2}\times10\times a \times b\sqrt{a}+ab\times6\sqrt{a}-5\times2\times a\sqrt{b} \\ = 5ab\sqrt{a}+6ab\sqrt{a}-10a\sqrt{b} \\= 11ab\sqrt{a}-10a\sqrt{b}
$$

## Dividing Surds

- To divide surds, divide the expression under the radical signs

$$
\frac{\sqrt{a}}{\sqrt{b}}=\sqrt{\frac{a}{b}}
$$

Where $a$ and $b$ are positive real numbers.

- When dividing surds it is best to simplify them (if possible) first. Once this has been done, the coefficients are divided next and then the surds are divided.

$$
\frac{m\sqrt{a}}{n\sqrt{b}} = \frac{m}{n}\sqrt{\frac{a}{b}}
$$

## Example

Simplify $\frac{9\sqrt{88}}{6\sqrt{99}}$

$$
=\frac{9}{6}\sqrt{\frac{88}{99}} \\= \frac{9}{8}\sqrt{\frac{8}{9}} \\ = \frac{9\times2\sqrt{2}}{6\times3} \\ =\frac{18\sqrt{2}}{18} \\ = \sqrt{2}
$$

Simplify $\frac{\sqrt{36xy}}{\sqrt{25x^{9}y^{11}}}$

$$
=\frac{6\sqrt{xy}}{5\sqrt{x^{8}\times x \times y^{10}\times y}} \\ = \frac{6\sqrt{xy}}{5x^{4}y^{5}\sqrt{}xy} \\ = \frac{6}{5x^{4}y^{5}}
$$

## Rationalising the denominator

- When the denominator of a fraction is a surd it can be turned into a rational number through multiplication.

$$
\frac{\sqrt{a}}{\sqrt{b}} = \frac{\sqrt{a}}{\sqrt{b}} \times \frac{\sqrt{b}}{\sqrt{b}} = \frac{\sqrt{ab}}{b} 
$$

## Example

Simplify $\frac{2\sqrt{12}}{3\sqrt{54}}$

$$
= \frac{2\sqrt{4\times3}}{3\sqrt{9\times6}} \\ = \frac{2\times2\sqrt{3}}{3\times3\sqrt{6}} \\ = \frac{4\sqrt{3}}{9\sqrt{6}} \\ = \frac{4\sqrt{3}}{9\sqrt{6}} \times \frac{\sqrt{6}}{\sqrt{6}} \\ = \frac{4\sqrt{18}}{9\times6} \\ = \frac{4\sqrt{9\times2}}{9\times6} \\ \frac{4\times3\sqrt{2}}{54} \\ = \frac{12\sqrt{2}}{54} \\ = \frac{2\sqrt{2}}{9}
$$